Formalize concurrent execution /w two-tier semantics
The concurrent execution of nodes is now modeled using a two-tiered
semantics. There are two sets of (related) inference rules: a thread-local
semantics and a global semantics. The thread-local semantics defines
execution of a command by a particular node. The global semantics
non-deterministically selects which node should execute, and updates the
state by using the thread-local semantics with the chosen node. This
two-tier semantics is important for the noninterference proof because it
gives us a way to model the fact that nodes can execute with an
arbitrary interleaving, and we want to show that there are no
information leaks regardless of scheduling (aside from perhaps
secheduling side channels).

The thread-local semantics closely resembles that of an imperative
programming language. A key difference though is that in order to be
language-agnostic (we cannot model the code that actually runs inside a
node aside from execution of the ABI calls) the semantics does not
contain usual constructs for control flow (like sequential composition
or loops). Instead, after any command is executed, a new command is
chosen nondeterministically (though the update to this command happens
in the global semantics). This models the fact that a node can
execute arbitrary code aside from the ABI calls in between calls to the
ABI. The choice of next command to execute is nondeterministic because
the next command does change, but there are no premises about the new
command in the inference rule.

The global semantics _nondeterministically_ chooses the thread to execute
because there are no premises about the thread that is used in the
thread-local semantics.

This two-tier semantics is inspired by "Secure Information Flow in a
Multi-threaded Imperative Langiage" by Smith and Volpano '98
(http://web.cs.ucla.edu/~palsberg/tba/papers/smith-volpano-popl98.pdf).
This same approach of modeling concurrent execution using a two-tier
semantics is also taken in "Compositional Non-interference for
Concurrent Programs via Separation and Framing."

experimental/ni_coq/vfiles/RuntimeModel.v
@@ -2,6 +2,7 @@ Require Import OakIFC.Lattice.
 Require Import OakIFC.Parameters.
 Require Import OakIFC.GenericMap.
 Require Import List.
+Import ListNotations.
 Require Import Coq.Sets.Ensembles.
 
 (* Ensembles don't have implicit type params and these lines fix that *)
@@ -17,37 +18,27 @@ Record channel := Chan {
     ms: list message
 }.
 
-(* Internal actions that nodes do other than ABI calls *)
-Inductive internal_cmd: Type :=
-    | IntRecvErr: internal_cmd (* TODO distinguish errors *)
-    | IntOther: internal_cmd
-    | IntRecvMesg (m: message): internal_cmd.
-
 (* ABI Calls *)
 Inductive call: Type :=
     | WriteChannel (h: handle) (m: message): call
-    | Internal (cmd: internal_cmd): call.
+    | ReadChannel (h: handle): call
+    | Internal: call.
 
 Record node := Node {
     nlbl: level;
-    calls: list call;
-    hans: Ensemble handle
+    hans: Ensemble handle;
+    ncall: call
 }.
-
-(* TODO: unsure if records or inductives are better for proofs.
-records are better for spec writing.
-also consider using a finite set of nodes rather than a map from
-node ids to nodes since node ids are not real anyway *)
 
 Instance Knid: KeyT := {
     t := node_id; 
     eq_dec := dec_eq_nid;
 }.
-Definition node_state := tg_map Knid node.
 Instance Khandle: KeyT := {
     t := handle;
     eq_dec := dec_eq_h;
 }.
+Definition node_state := tg_map Knid node.
 Definition chan_state := tg_map Khandle channel.
 Record state := State {
     nodes: node_state;
@@ -55,25 +46,24 @@ Record state := State {
 }.
 
 (*============================================================================
+* Empty
+============================================================================*)
+Definition empty_chan := {| clbl := top; ms := []; |}.
+Definition empty_node := {|
+        nlbl := top;
+        hans := Empty_set handle;
+        ncall := Internal;
+    |}.
+Definition empty_state := {| 
+        nodes := ( _ !-> empty_node);
+        chans := ( _ !-> empty_chan);
+    |}.
+
+(*============================================================================
 * Utils
 ============================================================================*)
 Definition chan_append (c: channel)(m: message): channel :=
     {| clbl := c.(clbl); ms := (m :: c.(ms)) |}.
-
-Definition node_push_c (n: node)(c: call): node :=
-    match n with | Node l cs hs => Node l (c :: cs) hs end .
-
-Definition is_node_call (n: node)(c: call): Prop :=
-    match n.(calls) with
-        | c :: _ => True
-        | _ => False
-    end.
-
-Definition node_pop_cmd (n: node): node :=
-    match n.(calls) with
-        | c :: cs' => Node n.(nlbl) n.(calls) n.(hans)
-        | _ => n
-    end.
 
 Definition state_upd_node (nid: node_id)(n: node)(s: state): state :=
     {| 
@@ -87,38 +77,47 @@ Definition state_upd_chan (h: handle)(ch: channel)(s: state): state :=
         chans := tg_update s.(chans) h ch;
     |}.
 
-Definition state_pop_caller (nid: node_id)(s: state): state := 
-    state_upd_node nid (node_pop_cmd (s.(nodes) nid)) s.
-
-(*
-Definition opt_match {A: Type}(o: option A)(a: A): Prop :=
-    match o with | Some a => True | _ => False end.
-*)
-
 (*============================================================================
 * Single Call Semantics
 ============================================================================*)
 
-Inductive step_call: node_id -> call -> state -> state -> Prop :=
-    | SWriteSucc caller_id han msg s
-        (H0: In (s.(nodes) caller_id).(hans) han)
-        (H2: (s.(nodes) caller_id).(nlbl) << (s.(chans) han).(clbl)):
-        step_call caller_id (WriteChannel han msg) s 
+(* step for a single node (which can be thought of as a thread) *)
+Inductive step_node: node_id -> state -> state -> Prop :=
+    | SWriteSucc s id n han msg
+        (H0: (s.(nodes) id) = n)
+        (H1: n.(ncall) = WriteChannel han msg)
+        (H1: In n.(hans) han)
+        (H2: n.(nlbl) << (s.(chans) han).(clbl)):
+        step_node id s
             (state_upd_chan han (chan_append (s.(chans) han) msg) s).
-    (*
-    | SWriteLblErr caller_id han chan msg s
-        (H0: In (s.(nodes) caller_id).(hans) han)
-        (H1: opt_match (s.(chans) han) chan)
-        (H2: ~((s.(nodes) caller_id).(nlbl) << chan.(clbl))):
-        step_call caller_id (WriteChannel han msg) s 
-            ( let n' := (node_push_c (s.(nodes) caller_id)
-                (Internal IntRecvErr)) in
-            state_upd_node caller_id n' s).
-    *)
+    (* TODO all the other calls *)
 
+(* step for the full system (which picks a thread to execute and is
+non-deterministic). This is needed in addition to step_node, because
+we should show that regardless of the thread ordering, there are no information
+leaks. *)
 Inductive step_system: state -> state -> Prop :=
-    | ValidStep caller_id caller call s s_pop s'
-        (H1: is_node_call caller call)
-        (H3: s_pop = state_pop_caller caller_id s)
-        (H4: step_call caller_id call s_pop s'):
+    (* possibly also a termination case *)
+    | ValidStep id s s'
+        (H1: step_node id s s'):
         step_system s s'.
+
+(* Traces are sequences of states modeling entire executions *)
+(* Noninterference definitions are defined by comparing "any two" executions *)
+Definition global_state: Type := state.
+Definition trace := list global_state.
+
+Definition last_state (t: trace)(s: state): Prop :=
+    match t with
+        | [] => False
+        | x :: t' => s = x
+    end.
+
+Inductive valid_trace (init: state): trace -> Prop :=
+    | VTOne: (valid_trace init [init] )
+    | VTAdd (s s': state)(t: trace)
+            (H0: valid_trace init t )
+            (H1: last_state t s')
+            (H2: step_system s s):
+            valid_trace init (s' :: t).
+
