experimental/ni_coq/vfiles/LowEquivalences.v
@@ -3,6 +3,22 @@ Require Import OakIFC.Parameters.
 Require Import Coq.Lists.List.
 Import ListNotations.
 
+(*=============================================================================
+* Low Equivalences
+=============================================================================*)
+(* 
+This file defines "low equivalence relations" over various pieces of state.
+These are auxiliary definitions for defining the security condition.
+A low-equivalence relation holds for a particular security level ell, and a pair
+of state objects s1, s2 whenever the "appear the same" from the perspective of
+an observer at the level ell. For example, if the state objects are channels,
+an observer with security label "Alice" can see the contents of channels with
+label "Alice" (or any other ell s.t. ell flowsTo Alice), so channels with such
+labels are related if their contents are equal. By contrast, Alice should not be
+able to see channels labeled "Bob", so _any_ pair of channels with this label
+are related even if their contents differ.
+*)
+
 Inductive chan_low_eq: level -> channel -> channel -> Prop :=
     | ChEq ell ch1 ch2 (H: ch1 = ch2): chan_low_eq ell ch1 ch2
     | ChNoFlow ell ch1 ch2
@@ -30,20 +46,47 @@ Definition state_low_eq (ell: level)(s1 s2: state): Prop :=
     (node_state_low_eq ell s1.(nodes) s2.(nodes)) /\
         (chan_state_low_eq ell s1.(chans) s2.(chans)).
 
-Definition trace := list state.
 
+(* 
+Usually, the low-equivalence relation over traces of states are where we can
+tell if the noninterference definition is timing sensitive. The Oak runtime
+does not prevent timing channels, and we actually need to do more work when
+specifying the theorem to allow them in the security condition. 
+
+A straightforward trace low-equivalence definition might say that
+t1 =L t2 <-> forall i, t1[i] =L t2[i]. But if one of the traces (say t2) 
+takes longer to execute code for some node _other than L_, it will "stutter"
+with several states in a row that are all low-equivalent because just the "high
+parts" that L can't see could have changed.
+
+This "up to high stutter" definition can be thought of as "collapsing" adjacent
+low-equivalent states in each trace and then comparing them after they are
+collapsed. The "collapsing" constructors are AddEqR and AddEqL.
+
+Trace_low_eq is the simpler definition. It is likely sufficient for trace
+propertries about executing a single node in serial.
+
+Stut_trace_low_eq is the "up to high stutter" definition.
+*)
 Inductive trace_low_eq: level -> trace -> trace -> Prop :=
     | NilEQ ell: trace_low_eq ell [] []
     | AddBoth ell x y t1 t2 
         (H1: trace_low_eq ell t1 t2)
         (H2: state_low_eq ell x y):
-        trace_low_eq ell (x::t1) (y::t2)
-    | AddEqR ell x y t1 t2 
-        (H1: trace_low_eq ell t1 (y::t2))
+        trace_low_eq ell (x::t1) (y::t2).
+
+Inductive stut_trace_low_eq: level -> trace -> trace -> Prop :=
+    | SNilEQ ell: stut_trace_low_eq ell [] []
+    | SAddBoth ell x y t1 t2 
+        (H1: stut_trace_low_eq ell t1 t2)
         (H2: state_low_eq ell x y):
-        trace_low_eq ell t1 (x::y::t2)
-    | AddEqL ell x y t1 t2 
-        (H1: trace_low_eq ell (y::t1) t2)
+        stut_trace_low_eq ell (x::t1) (y::t2)
+    | SAddEqR ell x y t1 t2 
+        (H1: stut_trace_low_eq ell t1 (y::t2))
         (H2: state_low_eq ell x y):
-        trace_low_eq ell (x::y::t1) t2.
+        stut_trace_low_eq ell t1 (x::y::t2)
+    | SAddEqL ell x y t1 t2 
+        (H1: stut_trace_low_eq ell (y::t1) t2)
+        (H2: state_low_eq ell x y):
+        stut_trace_low_eq ell (x::y::t1) t2.
 
