experimental/ni_coq/vfiles/StepUnwind.v
@@ -1,0 +1,97 @@
+Require Import OakIFC.RuntimeModel.
+Require Import OakIFC.Parameters.
+Require Import OakIFC.LowEquivalences.
+Require Import Coq.Lists.List.
+Require Import OakIFC.GenericMap.
+Import ListNotations.
+
+Theorem chan_upd_preserves_nodes: forall h ch s,
+    (state_upd_chan h ch s).(nodes) = s.(nodes).
+    intros; simpl; reflexivity.
+Qed.
+
+Theorem chan_append_unwind: forall ell m ch1 ch2,
+    (chan_low_eq ell ch1 ch2) ->
+    (chan_low_eq ell (chan_append ch1 m) (chan_append ch2 m)). 
+Proof.
+    intros. inversion H. 
+    constructor. rewrite H0. reflexivity.
+    constructor 2.
+    apply H1. apply H2.
+Qed. 
+
+Theorem leq_ch_upd_preserves_sleq: forall (ell: level)
+    (h:handle)(ch1 ch2: channel)(s1 s2:state),
+    (chan_low_eq ell ch1 ch2) ->
+    (state_low_eq ell s1 s2) ->
+    (state_low_eq ell 
+        (state_upd_chan h ch1 s1)
+        (state_upd_chan h ch2 s2)).
+Proof.
+    intros.
+    inversion H.
+        (* ch1 = ch2 *)
+        - rewrite H1. unfold state_low_eq. split.
+            (* node_state *)
+            rewrite chan_upd_preserves_nodes.
+            rewrite chan_upd_preserves_nodes.
+            apply H0.
+            (* chan_state *)
+            unfold chan_state_low_eq. intros.
+            destruct (dec_eq_h h h0).
+                (* h = h0 *)
+                + rewrite e. unfold state_upd_chan.
+                simpl. rewrite upd_eq. rewrite upd_eq.
+                constructor. reflexivity.
+                (* h <> h0 *)
+                + unfold state_upd_chan. simpl. 
+                rewrite upd_neq. rewrite upd_neq.
+                apply H0. apply n. apply n.
+        (* ~(ch1.l flowsTo ell) /\ ~(ch2.l flowsTo ell) *)
+        - unfold state_low_eq. split.
+            (* node_state *)
+            rewrite chan_upd_preserves_nodes.
+            rewrite chan_upd_preserves_nodes.
+            apply H0.
+            (* chan_state *)
+            unfold chan_state_low_eq. intros. destruct (dec_eq_h h h0).
+                (* h = h0 *)
+                + rewrite e. unfold state_upd_chan. simpl.
+                rewrite upd_eq. rewrite upd_eq.
+                constructor 2. apply H1. apply H2.
+                (* h <> h0 *)
+                + unfold state_upd_chan. simpl. 
+                rewrite upd_neq. rewrite upd_neq.
+                apply H0. apply n. apply n.
+Qed.
+
+Theorem low_eq_step: forall (ell: level)(s1 s2 s1' s2': state)
+        (n: node_id),
+    (state_low_eq ell s1 s2) ->
+    (step_node n s1 s1') ->
+    (step_node n s2 s2') ->
+    (state_low_eq ell s1' s2').
+Proof.
+    intros. inversion H0. inversion H1.
+    subst. 
+        (* commands don't necessarily match in the two 
+        * executions which complicates proof.
+        * in principle, this could probably be done by reasoning
+        * about the cases where the node being executed is / is not
+        * observable, write a separate theorem showing that the
+        * command _is_ the same when the node is observable, and that
+        * it does not matter what the command is if the node is above ell. 
+        *) 
+        (* the proofs will likely be simplified a lot by moving parts of a node
+        * into a single global state *)
+(*
+        destruct c.
+    - inversion H0.
+    - inversion H0. inversion H1.
+    apply leq_ch_upd_preserves_sleq.
+    apply chan_append_unwind.
+    apply H. apply H.
+    - inversion H0. 
+    - inversion H0.
+*)
+Admitted.
